attempt on proving reflection and fixing typing interpreter

theories/type_checker.v
@@ -177,21 +177,32 @@ Definition c_types_agree (ct : checker_type) (ts' : list value_type) : bool :=
   | CT_bot => false
   end.
 
-Fixpoint check_single (C : t_context) (be : basic_instruction) (ts : checker_type) {struct be} : checker_type :=
-  let check := fix check (C : t_context) (es : list basic_instruction) (ts : checker_type) {struct es} : checker_type :=
-      match es with
-      | [::] => ts
-      | e :: es' =>
-        match ts with
-        | CT_bot => CT_bot
-        | _ => check C es' (check_single C e ts)
-        end
-      end in
-  let b_e_type_checker C (es : list basic_instruction) tf :=
-       match tf with
-       | Tf tn tm =>
-         c_types_agree (check C es (CT_type tn)) tm
-       end in 
+(* TODO ----
+  An attempt to fix the type checker. However, after getting to this point, we are in
+    the same situation as the actual interpreter -- the following does not work as is
+    due to syntactic termination, so either we add a fuel or use some other methods.
+  
+  I don't want to use fuel every time and want to learn how to do this properly. There
+    is a reference which seems to be a good learning source:
+      http://adam.chlipala.net/cpdt/html/Cpdt.GeneralRec.html
+  This uses merge sort as an example, and gives two approaches: 
+      - well-founded recursion, or
+      - a monadic approach.
+  The second might be what Martin is trying to do. I'm trying to learn from this 
+    source currently.
+ *)
+
+Fixpoint check (C : t_context) (es : list basic_instruction) (ts : checker_type) {struct es} : checker_type :=
+  match es with
+  | [::] => ts
+  | e :: es' =>
+    match ts with
+    | CT_bot => CT_bot
+    | _ => check C es' (check_single C e ts)
+    end
+  end
+
+with check_single (C : t_context) (be : basic_instruction) (ts : checker_type) {struct be} : checker_type :=
   match be with
   | EConst v => type_update ts [::] (CT_type [::typeof v])
   | Unop_i t _ =>
@@ -364,22 +375,9 @@ Fixpoint check_single (C : t_context) (be : basic_instruction) (ts : checker_typ
     if tc_memory C != None
     then type_update ts [::CTA_some T_i32] (CT_type [::T_i32])
     else CT_bot
-  end.
+  end
 
-
-(* TODO: try to avoid repetition *)
-Fixpoint check (C : t_context) (es : list basic_instruction) (ts : checker_type) {struct es} : checker_type :=
-  match es with
-  | [::] => ts
-  | e :: es' =>
-    match ts with
-    | CT_bot => CT_bot
-    | _ => check C es' (check_single C e ts)
-    end
-  end.
-
-(* TODO: try to avoid repetition *)
-Definition b_e_type_checker (C : t_context) (es : list basic_instruction) (tf : function_type) : bool :=
+with b_e_type_checker (C : t_context) (es : list basic_instruction) (tf : function_type) {struct es}: bool :=
   match tf with
   | Tf tn tm => c_types_agree (check C es (CT_type tn)) tm
   end.
