theories/type_checker_reflects_typing.v
@@ -10,6 +10,13 @@ Unset Printing Implicit Defensive.
 
 Require Import operations typing type_checker.
 
+Lemma ct_suffix_empty: forall l,
+    ct_suffix [::] l.
+Proof.
+  move => l. unfold ct_suffix => /=.
+  rewrite subn0. apply/eqP. by apply drop_size.
+Qed.
+
 Lemma wasm_type_checker_reflects_typing:
   forall C es,
     reflect (cl_typing_self C es) (cl_type_check C es).
@@ -22,8 +29,25 @@ Proof.
       admit.
     + move => _. by apply cl_typing_host.
   - apply ReflectF. move => tc_prop.
+    assert (cl_type_check C es = true) as HTest; last by rewrite tc_bool in HTest.
+    clear tc_bool.
+    unfold cl_typing_self in tc_prop.
     inversion tc_prop; subst => //=.
-    + 
+    unfold c_types_agree.
+    clear H5.
+    (* This is important as otherwise Coq will fail to remember this information
+         and the proof cannot be done otherwise. It's in SF but this is also a 
+         good reference:
+https://stackoverflow.com/questions/4519692/keeping-information-when-using-induction
+    *)
+    remember (Tf [::] t2s) as tf.
+    clear tc_prop.
+    induction H2; subst => //.
+    + inversion Heqtf. by apply/eqP.
+    + simpl. by rewrite ct_suffix_empty.
+    + inversion Heqtf. by apply/eqP.
+    + simpl.
+
     
 Admitted. (* TODO *)
 
